.lake/build/ir/URFSpine/SpineSNFCanonicalRep.c
@@ -1,6 +1,6 @@
 // Lean compiler output
 // Module: URFSpine.SpineSNFCanonicalRep
-// Imports: public import Init public import Mathlib.Data.List.Sort public import Mathlib.Data.List.Basic public import URFSpine.Core.Artifact
+// Imports: public import Init public import Mathlib.Data.List.Sort
 #include <lean/lean.h>
 #if defined(__clang__)
 #pragma clang diagnostic ignored "-Wunused-parameter"
@@ -13,70 +13,27 @@
 #ifdef __cplusplus
 extern "C" {
 #endif
-LEAN_EXPORT lean_object* lp_urf__spine_URFSpine_key___boxed(lean_object*);
-LEAN_EXPORT uint8_t lp_urf__spine_URFSpine_leA(lean_object*, lean_object*);
-uint8_t l_String_decLE(lean_object*, lean_object*);
 lean_object* l_List_MergeSort_Internal_mergeSortTR_u2082___redArg(lean_object*, lean_object*);
-static lean_object* lp_urf__spine_URFSpine_SNF___closed__0;
-LEAN_EXPORT lean_object* lp_urf__spine_URFSpine_SNF(lean_object*);
-LEAN_EXPORT lean_object* lp_urf__spine_URFSpine_key(lean_object*);
-LEAN_EXPORT lean_object* lp_urf__spine_URFSpine_leA___boxed(lean_object*, lean_object*);
-LEAN_EXPORT lean_object* lp_urf__spine_URFSpine_key(lean_object* x_1) {
+LEAN_EXPORT lean_object* lp_urf__spine_URFSpine_SNF(lean_object*, lean_object*, lean_object*);
+LEAN_EXPORT lean_object* lp_urf__spine_URFSpine_SNF___redArg(lean_object*, lean_object*);
+LEAN_EXPORT lean_object* lp_urf__spine_URFSpine_SNF(lean_object* x_1, lean_object* x_2, lean_object* x_3) {
 _start:
 {
-lean_inc_ref(x_1);
-return x_1;
-}
-}
-LEAN_EXPORT lean_object* lp_urf__spine_URFSpine_key___boxed(lean_object* x_1) {
-_start:
-{
-lean_object* x_2; 
-x_2 = lp_urf__spine_URFSpine_key(x_1);
-lean_dec_ref(x_1);
-return x_2;
-}
-}
-LEAN_EXPORT uint8_t lp_urf__spine_URFSpine_leA(lean_object* x_1, lean_object* x_2) {
-_start:
-{
-uint8_t x_3; 
-x_3 = l_String_decLE(x_1, x_2);
-return x_3;
-}
-}
-LEAN_EXPORT lean_object* lp_urf__spine_URFSpine_leA___boxed(lean_object* x_1, lean_object* x_2) {
-_start:
-{
-uint8_t x_3; lean_object* x_4; 
-x_3 = lp_urf__spine_URFSpine_leA(x_1, x_2);
-lean_dec_ref(x_2);
-lean_dec_ref(x_1);
-x_4 = lean_box(x_3);
+lean_object* x_4; 
+x_4 = l_List_MergeSort_Internal_mergeSortTR_u2082___redArg(x_3, x_2);
 return x_4;
 }
 }
-static lean_object* _init_lp_urf__spine_URFSpine_SNF___closed__0() {
+LEAN_EXPORT lean_object* lp_urf__spine_URFSpine_SNF___redArg(lean_object* x_1, lean_object* x_2) {
 _start:
 {
-lean_object* x_1; 
-x_1 = lean_alloc_closure((void*)(lp_urf__spine_URFSpine_leA___boxed), 2, 0);
-return x_1;
-}
-}
-LEAN_EXPORT lean_object* lp_urf__spine_URFSpine_SNF(lean_object* x_1) {
-_start:
-{
-lean_object* x_2; lean_object* x_3; 
-x_2 = lp_urf__spine_URFSpine_SNF___closed__0;
-x_3 = l_List_MergeSort_Internal_mergeSortTR_u2082___redArg(x_1, x_2);
+lean_object* x_3; 
+x_3 = l_List_MergeSort_Internal_mergeSortTR_u2082___redArg(x_2, x_1);
 return x_3;
 }
 }
 lean_object* initialize_Init(uint8_t builtin);
 lean_object* initialize_mathlib_Mathlib_Data_List_Sort(uint8_t builtin);
-lean_object* initialize_mathlib_Mathlib_Data_List_Basic(uint8_t builtin);
-lean_object* initialize_urf__spine_URFSpine_Core_Artifact(uint8_t builtin);
 static bool _G_initialized = false;
 LEAN_EXPORT lean_object* initialize_urf__spine_URFSpine_SpineSNFCanonicalRep(uint8_t builtin) {
 lean_object * res;
@@ -88,14 +45,6 @@ lean_dec_ref(res);
 res = initialize_mathlib_Mathlib_Data_List_Sort(builtin);
 if (lean_io_result_is_error(res)) return res;
 lean_dec_ref(res);
-res = initialize_mathlib_Mathlib_Data_List_Basic(builtin);
-if (lean_io_result_is_error(res)) return res;
-lean_dec_ref(res);
-res = initialize_urf__spine_URFSpine_Core_Artifact(builtin);
-if (lean_io_result_is_error(res)) return res;
-lean_dec_ref(res);
-lp_urf__spine_URFSpine_SNF___closed__0 = _init_lp_urf__spine_URFSpine_SNF___closed__0();
-lean_mark_persistent(lp_urf__spine_URFSpine_SNF___closed__0);
 return lean_io_result_mk_ok(lean_box(0));
 }
 #ifdef __cplusplus
